\documentclass[letterpaper, 12pt]{article}

\usepackage{graphicx}
\usepackage{longtable}
\usepackage{rotating}
\usepackage{dcolumn}
\usepackage{listings}
\usepackage{subfiles}
\usepackage{amsmath}

% Code listing commands
\lstset{language=R,
basicstyle=\scriptsize\ttfamily,
commentstyle=\ttfamily,
numbers=left,
numberstyle=\footnotesize,
stepnumber=1,
numbersep=5pt,
showspaces=false,
showstringspaces=false,
showtabs=false,
frame=single,
tabsize=2,
captionpos=b,
breaklines=true,
breakatwhitespace=false,
title=\lstname,
escapeinside={},
keywordstyle={},
morekeywords={}
}

\begin{document}
\title{ARE213 Problem Set \#2A}
\author{Peter Alstone \& Frank Proulx}
\maketitle

\section{Problem \#1}
\subsection{Part A}
Here we will consider the within estimator, as suggested. This suggests that we want to find $\widehat{\beta_{FE}}$ by running the following regression:
\begin{equation}
\ddot{Y_{it}} = \ddot{X_{it}}\widehat{\beta_{FE}} + \ddot{\epsilon_{it}}
\end{equation}
Where $\ddot{Y_{it}}=Y_{it}-\bar{Y_i}$, $\ddot{X_{it}}=X_{it}-\bar{X_i}$, $\bar{Y_i}=\frac{1}{T}\sum_{t=1}^TY_{it}$, and $\bar{X_i}=\frac{1}{T}\sum_{t=1}^TX_{it}$.
Based on OLS, our fixed effects estimator is:
\begin{equation}
\widehat{\beta_{FE}}=(\ddot{X'_{it}}\ddot{X_{it}})^{-1}\ddot{X'_{it}}\ddot{Y_{it}} %His notes say you ``don't have to invert the mega-matrix'', so I might be doing this wrong.
\end{equation}

We know that $\ddot{X_{i}}=\boldsymbol{A}X_i$ and $\ddot{Y_{i}}=\boldsymbol{A}Y_{i}$, so
\begin{equation}
\widehat{\beta_{FE}} = (X'_{it}\boldsymbol{A}\boldsymbol{A}X_{it})^{-1} X_{it}\boldsymbol{A}\boldsymbol{A}Y_{it}
\end{equation}

However, since AA=A, and thus $\boldsymbol{AA}=\boldsymbol{A}$, this reduces to
\begin{equation}
\widehat{\beta_{FE}} = (X'_{it}\boldsymbol{A}X_{it})^{-1} X_{it} \boldsymbol{A} Y_{it}
\end{equation}

Given that T=2, this can be broken up as follows:





And looking at the first differences estimator, where we get $\widehat{\beta_{FD}}$ by running the regression
\begin{equation}
\Delta Y_{it} = \Delta X'_{it} \widehat{\beta_{FD}} + \Delta \epsilon_{it}
\end{equation}

where $\Delta Y_{it} = Y_{it} - Y_{it-1}$, $\Delta X_{it} = X_{it} - X_{it-1}$, and $\Delta \epsilon_{it} = \epsilon_{it} - \epsilon_{it-1}$.

Because we only have T=2, this differencing estimator can only be estimated for t=2, so we regress
\begin{align}
\Delta Y_{i2} = \Delta X'_{i2} \widehat{\beta_{FD}} + \Delta \epsilon_{i2} \\
Y_{i2}-Y_{i1} = (X_{i2}-X_{i1})'\widehat{\beta_{FD}} + \epsilon_{i2}-\epsilon_{i1}
\end{align}

thus, our first difference estimator is
\begin{equation}
\widehat{\beta_{FD}}=((X_{i2}-X_{i1})'(X_{i2}-X_{i1}))^{-1} (X_{i2}-X_{i1})'(Y_{i2}-Y_{i1})
\end{equation}





\end{document}
